progress

Veir/Data/LLVM/Int/Lemmas.lean
@@ -2,21 +2,106 @@ module
 
 import all Veir.Data.LLVM.Int.Basic
 import Veir.ForLean
+import Veir.Data.LLVM.Int.Simp
 
 open Veir.Data.LLVM
 
 namespace Veir.Data.LLVM.Int
 
+@[ext]
+structure IntBv (w : Nat) where
+  toBitVec : BitVec w
+  poison : Bool
+deriving DecidableEq
+
+/-- An `LLVM.Int w` is converted into a structure `IntBv`, where
+  the `poison` field indicates whether the `Int` is poison. -/
+def toIntBv (x : Int w) : IntBv w :=
+  match x with
+  | .val v => ⟨v, false⟩
+  | .poison => ⟨0#w, true⟩
+
+@[simp]
+theorem toIntBv_poison :
+    poison.toIntBv = ⟨0#w, true⟩ := by
+  simp [toIntBv]
+
+@[simp]
+theorem toIntBv_val :
+    (val v).toIntBv = ⟨v, false⟩ := by
+  simp [toIntBv]
+
+theorem BitVec.ne_iff_exists {x y : BitVec w} :
+    x ≠ y ↔ ∃ i, x.getLsbD i ≠ y.getLsbD i := by
+  constructor
+  · intro h
+    refine Nat.exists_testBit_ne_of_ne ?_
+    simp [← BitVec.toNat_inj] at h
+    simp [h]
+  · intro h
+    obtain ⟨i, hi⟩ := h
+    simp
+    exact Ne.symm fun a => hi (congrFun (congrArg BitVec.getLsbD (id (Eq.symm a))) i)
+
+theorem BitVec.append_eq_iff {x y : BitVec w} {z : BitVec v} :
+    x ++ z = y ++ z ↔ x = y := by
+  constructor
+  · intro h
+    exact (BitVec.append_left_inj z).mp h
+  · intro h
+    exact (BitVec.append_left_inj z).mpr h
+
+theorem Int.toIntBv.inj {w : Nat} : ∀ {x y : Int w}, x.toIntBv = y.toIntBv → x = y
+  | .val v,  .val v',  h => by
+    simp only [toIntBv, IntBv.mk.injEq, and_true] at h
+    simp [h]
+  | .poison, .poison, _ => rfl
+  | .val v,  .poison, h => by
+    simp [toIntBv] at h
+  | .poison, .val v,  h => by
+    simp [toIntBv] at h
+
+@[llvm_toBitVec]
+theorem int_inj (i1 i2 : Int w) :
+    i1 = i2 ↔ i1.toIntBv = i2.toIntBv := ⟨(· ▸ rfl), Int.toIntBv.inj⟩
+
 /- # add -/
 
-@[simp, grind =]
+@[llvm_toBitVec]
+theorem constant_val {w : Nat} (v : _root_.Int) :
+    (constant w v).toIntBv = ⟨BitVec.ofInt w v, false⟩ := by
+  simp [constant, toIntBv]
+
+theorem poison_of_forall (h : ∀ (y' : BitVec w), y = val y' → False) :
+    y = poison := by
+  rcases y
+  · case _ v =>
+    specialize h v
+    simp at h
+  · rfl
+
+@[grind =, llvm_toBitVec]
 theorem poison_add {w : Nat} (x : Int w) : add poison x = poison := by
   simp only [add, Id.run]
 
-@[simp, grind =]
+@[grind =, llvm_toBitVec]
 theorem add_poison {w : Nat} (x : Int w) : add x poison = poison := by
   simp only [add, Id.run]
   grind
+
+@[llvm_toBitVec]
+theorem add_val {w : Nat} {v v' : BitVec w} : add (val v) (val v') = val (v + v') := by
+  simp only [add, Id.run]
+  grind
+
+@[llvm_toBitVec]
+theorem add_int {w : Nat} (x y : Int w) :
+    (add x y).toIntBv =
+      if x.toIntBv.poison ∨ y.toIntBv.poison then ⟨0#w, true⟩
+        else ⟨x.toIntBv.toBitVec + y.toIntBv.toBitVec, false⟩ := by
+  simp [add, llvm_toBitVec, Id.run]
+  rcases x <;> rcases y
+  <;> simp [llvm_toBitVec]
 
 @[grind =]
 theorem add_assoc {w : Nat} (x y z : Int w) :
@@ -31,11 +116,11 @@ theorem add_comm {w : Nat} (x y : Int w) : add x y = add y x := by
 
 /- # mul -/
 
-@[simp, grind =]
+@[simp, grind =, llvm_toBitVec]
 theorem poison_mul {w : Nat} (x : Int w) : mul poison x = poison := by
   simp only [mul, Id.run]
 
-@[simp, grind =]
+@[simp, grind =, llvm_toBitVec]
 theorem mul_poison {w : Nat} (x : Int w) : mul x poison = poison := by
   simp only [mul, Id.run]
   grind
@@ -52,5 +137,10 @@ theorem mul_comm {w : Nat} {nsw nuw : Bool} (x y : Int w) :
   simp only [Id.run, Veir.Data.LLVM.Int.mul]
   cases x <;> cases y <;>
   simp [BitVec.mul_comm, BitVec.smulOverflow_comm, BitVec.umulOverflow_comm]
+
+theorem right_identity_zero_add':
+    (Veir.Data.LLVM.Int.add lhs (Veir.Data.LLVM.Int.constant 64 0)) = lhs := by
+  simp [llvm_toBitVec]
+  cases lhs <;> simp
 
 end Int
