Veir/Passes/Combines/Proofs.lean
@@ -1,4 +1,5 @@
 import Veir.Data.RISCV.Reg.Basic
+import Veir.Data.LLVM.Int.Basic
 import Veir.Data.RISCV.Reg.Lemmas
 
 /-!
@@ -6,6 +7,7 @@ import Veir.Data.RISCV.Reg.Lemmas
 -/
 
 namespace Veir.Data.RISCV
+namespace Veir.Data.LLVM
 
 
 /--
